tuning
* moving some theorems
* tuning theory imports
* deleting some comments

Weidenbach_Book/Array_Array_List.thy
@@ -686,4 +686,90 @@ lemma arrayO_raa_empty_sz_init_lrl[sepref_fr_rules]:
     nat_assn\<^sup>k \<rightarrow>\<^sub>a arrayO_assn (arl_assn R)\<close>
   using arrayO_ara_empty_sz_code.refine unfolding arrayO_ara_empty_sz_init_lrl .
 
+
+definition (in -) shorten_take_ll where
+  \<open>shorten_take_ll L j W = W[L := take j (W ! L)]\<close>
+
+definition (in -) shorten_take_aa where
+  \<open>shorten_take_aa L j W =  do {
+      (a, n) \<leftarrow> Array.nth W L;
+      Array.upd L (a, j) W
+    }\<close>
+
+
+lemma Array_upd_arrayO_except_assn[sep_heap_rules]:
+  assumes
+    \<open>ba \<le> length (b ! a)\<close> and
+    \<open>a < length b\<close>
+  shows \<open><arrayO_except_assn (arl_assn R) [a] b bi
+           (\<lambda>r'. arl_assn R (b ! a) (aaa, n) * \<up> ((aaa, n) = r' ! a))>
+         Array.upd a (aaa, ba) bi
+         <\<lambda>r. \<exists>\<^sub>Ax. arrayO_assn (arl_assn R) x r * true *
+                    \<up> (x = b[a := take ba (b ! a)])>\<close>
+proof -
+  have [simp]: \<open>ba \<le> length l'\<close>
+    if
+      \<open>ba \<le> length (b ! a)\<close> and
+      aa: \<open>(take n l', b ! a) \<in> \<langle>the_pure R\<rangle>list_rel\<close>
+    for l' :: \<open>'b list\<close>
+  proof -
+    show ?thesis
+      using list_rel_imp_same_length[OF aa] that
+      by auto
+  qed
+  have [simp]: \<open>(take ba l', take ba (b ! a)) \<in> \<langle>the_pure R\<rangle>list_rel\<close>
+    if
+      \<open>ba \<le> length (b ! a)\<close> and
+      \<open>n \<le> length l'\<close> and
+      take: \<open>(take n l', b ! a) \<in> \<langle>the_pure R\<rangle>list_rel\<close>
+    for l' :: \<open>'b list\<close>
+  proof -
+    have [simp]: \<open>n = length (b ! a)\<close>
+      using list_rel_imp_same_length[OF take] that by auto
+    have 1: \<open>take ba l' = take ba (take n l')\<close>
+      using that by (auto simp: min_def)
+    show ?thesis
+      using take
+      unfolding 1
+      by (rule list_rel_take)
+  qed
+
+  have [simp]: \<open>heap_list_all_nth (arl_assn R) (remove1 a [0..<length p])
+           (b[a := take ba (b ! a)]) (p[a := (aaa, ba)]) =
+        heap_list_all_nth (arl_assn R) (remove1 a [0..<length p]) b p\<close>
+    for p :: \<open>('b array \<times> nat) list\<close> and l' :: \<open>'b list\<close>
+  proof -
+    show ?thesis
+      by (rule heap_list_all_nth_cong) auto
+  qed
+
+  show ?thesis
+    using assms
+    unfolding arrayO_except_assn_def
+    apply (subst (2) arl_assn_def)
+    apply (subst is_array_list_def[abs_def])
+    apply (subst hr_comp_def[abs_def])
+    apply (subst array_assn_def)
+    apply (subst is_array_def[abs_def])
+    apply (subst hr_comp_def[abs_def])
+    apply sep_auto
+    apply (subst arrayO_except_assn_array0_index[symmetric, of a])
+    apply (solves simp)
+    unfolding arrayO_except_assn_def array_assn_def is_array_def
+    apply (subst (3) arl_assn_def)
+    apply (subst is_array_list_def[abs_def])
+    apply (subst (2) hr_comp_def[abs_def])
+    apply (subst ex_assn_move_out)+
+    apply (rule_tac x=\<open>p[a := (aaa, ba)]\<close> in ent_ex_postI)
+    apply (rule_tac x=\<open>take ba l'\<close> in ent_ex_postI)
+    by (sep_auto simp: )
+qed
+
+lemma shorten_take_aa_hnr[sepref_fr_rules]:
+  \<open>(uncurry2 shorten_take_aa, uncurry2 (RETURN ooo shorten_take_ll)) \<in>
+     [\<lambda>((L, j), W). j \<le> length (W ! L) \<and> L < length W]\<^sub>a
+    nat_assn\<^sup>k *\<^sub>a nat_assn\<^sup>k *\<^sub>a (arrayO_assn (arl_assn R))\<^sup>d \<rightarrow> arrayO_assn (arl_assn R)\<close>
+  unfolding shorten_take_aa_def shorten_take_ll_def
+  by sepref_to_hoare sep_auto
+
 end
